Validate submission 02e18b13-7678-47f7-90dc-3a7182dc634d
Co-authored-by: fkiene <46886660+fkiene@users.noreply.github.com>

Challenge/Modexp/Submission/Proofs/Bytecode/Artifact.lean
@@ -1820,7 +1820,7 @@ def submissionInstructions : List Instr :=
  YulEvmCompiler.Instr.op (EvmSemantics.Operation.CompBit (EvmSemantics.Operation.CompareBitwiseOps.BYTE)),
  YulEvmCompiler.Instr.op (EvmSemantics.Operation.Dup { idx := 1 }),
  YulEvmCompiler.Instr.op (EvmSemantics.Operation.CompBit (EvmSemantics.Operation.CompareBitwiseOps.ISZERO)),
- YulEvmCompiler.Instr.push 2 2944,
+YulEvmCompiler.Instr.push 2 3027,
  YulEvmCompiler.Instr.op (EvmSemantics.Operation.StackMemFlow (EvmSemantics.Operation.StackMemFlowOps.JUMPI)),
  YulEvmCompiler.Instr.push 1 128,
  YulEvmCompiler.Instr.push 2 1789,
@@ -1873,9 +1873,25 @@ def submissionInstructions : List Instr :=
  YulEvmCompiler.Instr.push 2 1832,
  YulEvmCompiler.Instr.op (EvmSemantics.Operation.StackMemFlow (EvmSemantics.Operation.StackMemFlowOps.JUMP)),
  YulEvmCompiler.Instr.op (EvmSemantics.Operation.StackMemFlow (EvmSemantics.Operation.StackMemFlowOps.JUMPDEST)),
- YulEvmCompiler.Instr.push 2 1789,
- YulEvmCompiler.Instr.op (EvmSemantics.Operation.StackMemFlow (EvmSemantics.Operation.StackMemFlowOps.JUMP))]
-theorem submissionInstructions_count : submissionInstructions.length = 1846 := by
+YulEvmCompiler.Instr.push 2 3027,
+YulEvmCompiler.Instr.op (EvmSemantics.Operation.StackMemFlow (EvmSemantics.Operation.StackMemFlowOps.JUMP)),
+YulEvmCompiler.Instr.op (EvmSemantics.Operation.StackMemFlow (EvmSemantics.Operation.StackMemFlowOps.JUMPDEST)),
+YulEvmCompiler.Instr.op (EvmSemantics.Operation.Dup { idx := 7 }),
+YulEvmCompiler.Instr.push 1 1,
+YulEvmCompiler.Instr.op (EvmSemantics.Operation.CompBit (EvmSemantics.Operation.CompareBitwiseOps.EQ)),
+YulEvmCompiler.Instr.push 2 3040,
+YulEvmCompiler.Instr.op (EvmSemantics.Operation.StackMemFlow (EvmSemantics.Operation.StackMemFlowOps.JUMPI)),
+YulEvmCompiler.Instr.push 2 1789,
+YulEvmCompiler.Instr.op (EvmSemantics.Operation.StackMemFlow (EvmSemantics.Operation.StackMemFlowOps.JUMP)),
+YulEvmCompiler.Instr.op (EvmSemantics.Operation.StackMemFlow (EvmSemantics.Operation.StackMemFlowOps.JUMPDEST)),
+YulEvmCompiler.Instr.op (EvmSemantics.Operation.StackMemFlow (EvmSemantics.Operation.StackMemFlowOps.POP)),
+YulEvmCompiler.Instr.op (EvmSemantics.Operation.StackMemFlow (EvmSemantics.Operation.StackMemFlowOps.POP)),
+YulEvmCompiler.Instr.push 1 1,
+YulEvmCompiler.Instr.op (EvmSemantics.Operation.StopArith (EvmSemantics.Operation.StopArithOps.ADD)),
+YulEvmCompiler.Instr.push 2 1769,
+YulEvmCompiler.Instr.op (EvmSemantics.Operation.StackMemFlow (EvmSemantics.Operation.StackMemFlowOps.JUMP))
+]
+theorem submissionInstructions_count : submissionInstructions.length = 1861 := by
   decide
 
 theorem assemble_submissionInstructions :
